Charge!/src/Charge/ModularFunc/EmbedFunc.v
@@ -3,15 +3,18 @@ Require Import ExtLib.Data.Fun.
 Require Import ExtLib.Data.Nat.
 Require Import ExtLib.Data.Bool.
 Require Import ExtLib.Data.String.
+Require Import ExtLib.Tactics.
 Require Import ExtLib.Tactics.Consider.
 
 Require Import MirrorCore.TypesI.
 Require Import MirrorCore.syms.SymEnv.
+Require Import MirrorCore.syms.SymSum.
 Require Import MirrorCore.Lambda.Expr.
 Require Import MirrorCore.SymI.
 
 Require Import Charge.Logics.ILogic.
 Require Import Charge.Logics.ILEmbed.
+Require Import Charge.ModularFunc.Denotation.
 Require Import Charge.ModularFunc.ILogicFunc.
 
 Require Import Coq.Strings.String.
@@ -113,24 +116,8 @@ Section EmbedFuncInst.
     destruct x; destruct y; simpl; rewrite andb_true_iff;
     repeat rewrite rel_dec_correct; intuition congruence.
   Qed.
-  
-  Definition typ2_cast' (a b : typ)
-  	: (typD a -> typD b) -> typD (tyArr a b) := 
-  		fun f =>
-  		match eq_sym (typ2_cast a b) in _ = t return t with
-  			| eq_refl => f
-  		end.
 
-  Definition typ2_cast_bin (a b c : typ)
-  : (typD a -> typD b -> typD c) -> typD (tyArr a (tyArr b c)) :=
-    fun f =>
-      match eq_sym (typ2_cast a (tyArr b c)) in _ = t
-            return t with
-        | eq_refl => match eq_sym (typ2_cast b c) in _ = t
-                           return _ -> t with
-                       | eq_refl => f
-                     end
-        end.
+ Definition embedD t u (EIL : EmbedOp (typD t) (typD u)) := fun_to_typ (@embed _ _ EIL).
 
  Definition funcD (f : embed_func typ) : match typeof_embed_func f with
 							              | Some t => typD t
@@ -152,11 +139,7 @@ Section EmbedFuncInst.
 		       | None => unit
 		     end
         with
-	  | Some t0 =>
-            match eq_sym (typ2_cast t u) in _ = t return t
-            with
-              | eq_refl => @embed _ _ _
-            end
+	  | Some t0 => embedD t u t0
 	  | None => tt
         end
     end.
@@ -182,3 +165,155 @@ Section MakeEmbed.
 	Definition mkEmbed (t u : typ) P := App (fEmbed t u) P.
 
 End MakeEmbed.
+
+Section EmbedFuncOk.
+  Context {typ func : Type} {HO: EmbedFunc typ func}.
+  Context {RType_typ : RType typ} {RSym_func : RSym func}.
+  Context {RelDec_eq : RelDec (@eq typ)}.
+
+  Context {Typ2_tyArr : Typ2 _ Fun}.
+  Let tyArr : typ -> typ -> typ := @typ2 _ _ _ _.
+  
+  Variable gs : embed_ops.
+  
+  Class EmbedFuncOk := {
+    eilf_funcAsOk (f : func) e : embedS f = Some e -> 
+      forall t, funcAs f t = funcAs (RSym_func := RSym_embed_func _ gs) e t;
+    eilf_fEmbedOk t u : embedS (fEmbed t u) = Some (eilf_embed t u)
+  }.
+
+End EmbedFuncOk.
+
+Implicit Arguments EmbedFuncOk [[HO] [RType_typ] [RSym_func] [RelDec_eq] [Typ2_tyArr]].
+
+Section EmbedFuncBaseOk.
+  Context {typ func : Type} {HO: EmbedFunc typ func}.
+  Context {RType_typ : RType typ} {RSym_func : RSym func}.
+  Context {RelDec_eq : RelDec (@eq typ)}.
+
+  Context {Typ2_tyArr : Typ2 _ Fun}.
+  Let tyArr : typ -> typ -> typ := @typ2 _ _ _ _.
+  
+  Variable gs : embed_ops.
+
+  Global Program Instance EmbedFuncBaseOk : EmbedFuncOk (RSym_func := RSym_embed_func _ gs) typ (embed_func typ) gs := {
+    eilf_funcAsOk := fun _ _ _ _ => eq_refl;
+    eilf_fEmbedOk t u := eq_refl
+  }.
+
+End EmbedFuncBaseOk.
+
+Section EmbedFuncExprOk.
+  Context {typ func : Type} `{HOK : EmbedFuncOk typ func}.
+  Context {HROk : RTypeOk}.
+  Context {A : Type} {RSymA : RSym A}.
+
+  Lemma BILogicFunc_typeOk (f : func) (e : embed_func typ) (H : embedS f = Some e) :
+    typeof_sym f = typeof_embed_func _ gs e.
+  Proof.
+    admit.
+    (*
+    destruct HOK as [H1 H2 _ _ _ _ _ _ _].
+    specialize (H1 _ _ H).
+    destruct e; simpl in *;
+    remember (gs logic) as o;
+    destruct o; try
+    match goal with 
+      | |- typeof_sym ?f = Some ?t => 
+	 	specialize (H1 t);
+	 	simpl in H1;
+	 	unfold funcAs in H1; simpl in H1; rewrite <- Heqo, type_cast_refl in H1; [|apply _];
+	 	generalize dependent (symD f);
+	 	destruct (typeof_sym f); simpl; intros; [forward|]; inversion H1
+ 	end;
+ 	unfold funcAs in H1; simpl in H1; unfold empD in H1; rewrite <- Heqo in H1;
+ 	generalize dependent (symD f);
+ 	remember (typeof_sym f).
+ 	(destruct o; intros; [|]). specialize (H1 logic). forward. inv_all; subst.
+ 	specialize (H1 t); (rewrite type_cast_refl in H1; [|apply _]);
+ 	inversion H1. 
+*)
+  Qed.
+  (*
+  Lemma bilogicS_is_bilogic (f : func) (e : bilfunc typ) t df
+  	(H1 : bilogicS f = Some e) (H2 : funcAs f t = Some df) :
+    exists IL, gs (bilfunc_logic e) = Some IL.
+  Proof.
+    admit.
+    (*
+    pose proof (bilf_funcAsOk _ H1) as H; 
+    rewrite H in H2; clear H;
+    destruct e; simpl in *;
+    unfold funcAs in H2; simpl in H2;
+    (destruct (gs logic); [eexists; reflexivity | congruence]).
+*)
+  Qed.
+  *)
+  Lemma eilf_embed_type_eq (f : func) t u v df
+    (H1 : embedS f = Some (eilf_embed t u)) (H2 : funcAs f v = Some df) :
+    v = typ2 t u.
+  Proof.
+    rewrite (eilf_funcAsOk _ H1) in H2.
+    unfold funcAs in H2. simpl in *.
+    
+    
+    forward. 
+  Qed.
+
+  Existing Instance RSym_sum.
+
+  Global Program Instance EmbedFuncOkSumR : EmbedFuncOk typ ((A + func)%type) gs := {
+    eilf_funcAsOk := 
+      fun a f H t => 
+        match a with
+          | inl b => _
+          | inr b => _
+        end;
+    eilf_fEmbedOk t u := eilf_fEmbedOk (func := func) t u
+  }.
+  Next Obligation.
+    apply (eilf_funcAsOk (func := func)).
+    apply H.
+  Qed.
+
+  Global Program Instance EmbedFuncOkSumL : EmbedFuncOk typ ((func + A)%type) gs := {
+    eilf_funcAsOk := 
+      fun a f H t => 
+        match a with
+          | inl b => _
+          | inr b => _
+        end;
+    eilf_fEmbedOk t u := eilf_fEmbedOk (func := func) t u
+  }.
+  Next Obligation.
+    apply (eilf_funcAsOk (func := func)).
+    apply H.
+  Qed.
+
+End EmbedFuncExprOk.
+
+Section MakeEmbedSound.
+  Context {typ func : Type} `{HOK : EmbedFuncOk typ func}.
+  Context {HROk : RTypeOk} {Typ2_tyArrOk : Typ2Ok Typ2_tyArr}
+          {RSym_funcOk : RSymOk RSym_func0}.
+
+  Let tyArr : typ -> typ -> typ := @typ2 _ _ _ _.
+
+  Lemma mkEmbed_sound (t u : typ) (tus tvs : tenv typ) p EIL
+    (dp: ExprI.exprT tus tvs (typD t))
+    (Hgs : gs t u = Some EIL)
+    (Hp : exprD' tus tvs t p = Some dp) :
+    exprD' tus tvs u (mkEmbed t u p) = Some (exprT_App (fun _ _ => embedD _ _ _ EIL) dp).
+  Proof.
+    unfold mkEmbed; simpl.
+    autorewrite with exprD_rw; simpl; forward; inv_all; subst.
+    rewrite (ExprTac.exprD_typeof_Some _ _ _ p _ Hp).
+    autorewrite with exprD_rw; simpl; forward; inv_all; subst.
+    pose proof (eilf_fEmbedOk t u) as Ho.
+    pose proof (eilf_funcAsOk _ Ho) as H1.
+    rewrite H1. unfold funcAs; simpl.
+    rewrite Hgs. rewrite type_cast_refl; [reflexivity | apply _].
+  Qed.
+
+End MakeEmbedSound.
+  
