Charge!/src/Charge/ModularFunc/Denotation.v
@@ -1,0 +1,46 @@
+Require Import ExtLib.Data.Fun.
+Require Import ExtLib.Data.HList.
+Require Import ExtLib.Tactics.
+
+Require Import MirrorCore.TypesI.
+Require Import MirrorCore.ExprI.
+Require Import MirrorCore.Lambda.Expr.
+
+Section Denotation.
+  Context {typ : Type} {RType_typ : RType typ}.
+  Context {Typ2_tyArr : Typ2 _ Fun}.
+
+  Let tyArr := @typ2 _ _ _ _.
+
+  Definition fun_to_typ {a b : typ} (f : typD a -> typD b) : typD (tyArr a b) :=
+    eq_rect_r id f (typ2_cast a b).
+    
+  Definition typ_to_fun {a b : typ} (f : typD (tyArr a b)) : typD a -> typD b :=
+  fun x => (fun g : typD a -> typD b => g x)
+    (eq_rect (typD (typ2 a b)) id f (typD a -> typD b)
+       (typ2_cast a b)).
+    
+  Definition fun_to_typ2 {a b c : typ} (f : typD a -> typD b -> typD c) :=
+     fun_to_typ (fun x => fun_to_typ (f x)). 
+
+  Definition fun_to_typ3 {a b c d : typ} (f : typD a -> typD b -> typD c -> typD d) :=
+    fun_to_typ (fun x => fun_to_typ (fun y => fun_to_typ (f x y))).
+
+  Definition fun_to_typ4 {a b c d e : typ} (f : typD a -> typD b -> typD c -> typD d -> typD e) :=
+    fun_to_typ (fun x => fun_to_typ (fun y => fun_to_typ (fun z => fun_to_typ (f x y z)))).
+
+  Definition typ_to_fun2 {a b c : typ} (f : typD (tyArr a (tyArr b c))) : typD a -> typD b -> typD c :=
+    fun x => typ_to_fun (typ_to_fun f x).
+
+  Definition typ_to_fun3 {a b c d : typ} (f : typD (tyArr a (tyArr b (tyArr c d)))) : 
+	  typD a -> typD b -> typD c -> typD d :=
+    fun x y => typ_to_fun (typ_to_fun (typ_to_fun f x) y).
+
+  Lemma exprT_App_wrap tus tvs (t u : typ) (f : HList.hlist typD tus -> HList.hlist typD tvs -> typD t -> typD u) (a : exprT tus tvs (typD t)) :
+    exprT_App (fun us vs => fun_to_typ (f us vs)) a = fun us vs => (f us vs) (a us vs).
+  Proof.
+    unfold fun_to_typ, exprT_App, eq_rect_r, eq_sym, eq_rect.
+    forward.
+  Qed.
+
+End Denotation.
