Charge!/src/Charge/Tactics/Rtac/Subst.v
@@ -8,6 +8,7 @@ Require Import MirrorCore.TypesI.
 Require Import MirrorCore.RTac.RTac.
 Require Import MirrorCore.Lambda.RedAll.
 
+Require Import Charge.ModularFunc.Denotation.
 Require Import Charge.ModularFunc.BaseFunc.
 Require Import Charge.ModularFunc.OpenFunc.
 Require Import Charge.ModularFunc.ILogicFunc.
@@ -74,7 +75,7 @@ Print baseS.
 		match f with
 		  | App (App g e') y =>
 		  	match open_funcS g, baseS y with
-		  	  | Some (of_singleSubst), Some (pString v) => applySingleSubst e x v e'
+		  	  | Some of_single_subst, Some (pString v) => applySingleSubst e x v e'
 		  	  | _, _ => mkApplySubst t e f
 		  	end
 		  | _ => mkApplySubst t e f
@@ -101,17 +102,17 @@ Section PushSubst.
     match e with
     	| App (App g p) q =>
     		match ilogicS g with
-    			| Some (ilf_and l) => mkAnd l (pushSubst p l) (pushSubst q l)
-    			| Some (ilf_or l) => mkOr l (pushSubst p l) (pushSubst q l)
-    			| Some (ilf_impl l) => mkImpl l (pushSubst p l) (pushSubst q l)
+    			| Some (ilf_and l) => mkAnd l (pushSubst p t) (pushSubst q t)
+    			| Some (ilf_or l) => mkOr l (pushSubst p t) (pushSubst q t)
+    			| Some (ilf_impl l) => mkImpl l (pushSubst p t) (pushSubst q t)
     			| Some _ => mkApplySubst t e f
     			| None => match open_funcS g with
 		    			 | Some (of_ap t1 t2) => mkAp t1 t2 (pushSubst p (tyArr t1 t2))
-		    			             									 (pushSubst q t2)
+		    			             									 (pushSubst q t1)
 		    			 | Some _ => mkApplySubst t e f
 		    			 | _ => match bilogicS g with
-		    			          | Some (bilf_star l) => mkStar l (pushSubst p l) (pushSubst q l)
-		    			          | Some (bilf_wand l) => mkWand l (pushSubst p l) (pushSubst q l)
+		    			          | Some (bilf_star l) => mkStar l (pushSubst p t) (pushSubst q t)
+		    			          | Some (bilf_wand l) => mkWand l (pushSubst p t) (pushSubst q t)
 		    			 	      | _ => mkApplySubst t e f
 		    			 	    end
 		    		   end
@@ -194,12 +195,164 @@ Require Import FunctionalExtensionality.
         apply H.
       Qed.
 
-    Lemma exprT_App_wrap tus tvs (t u : typ) (f : HList.hlist typD tus -> HList.hlist typD tvs -> typD t -> typD u) (a : exprT tus tvs (typD t)) :
-      exprT_App (fun us vs => fun_to_typ _ (f us vs)) a = fun us vs => (f us vs) (a us vs).
-    Proof.
-      unfold fun_to_typ, exprT_App, eq_rect_r, eq_sym, eq_rect.
-      forward.
-    Qed.
+Locate exprT_App.
+
+  Lemma Rcast_option_inj (t u : typ) r (a : typD t) (b : typD u)
+    (H : Rcast option r (Some a) = Some b) :
+    b = Rcast id r a.
+  Proof.
+    clear -H.
+    unfold Rcast, Relim, Rsym, eq_sym in *.
+    destruct r; inv_all; subst. reflexivity.
+  Qed.
+
+  Lemma Rcast_id t f : 
+    Rcast id (Rrefl t) f = f.
+  Proof.
+    reflexivity.
+  Qed.
+
+  Ltac clear_eq := 
+    match goal with 
+      | H : ?x = ?x |- _ => clear H
+    end.
+    
+  Ltac r_inj H :=
+      first [
+        let H1 := fresh "H" in let H2 := fresh "H" in
+          apply typ2_inj in H as [H1 H2]; [unfold Rty in H1, H2; r_inj H1; r_inj H2 | apply _] |
+        repeat subst].
+    
+Ltac forward_step :=
+  match goal with 
+    | H : Some _ = baseS _ |- _ =>  symmetry in H
+    | H : Some _ = embedS _ |- _ =>  symmetry in H
+    | H : Some _ = open_funcS _ |- _ =>  symmetry in H
+    | H : Some _ = bilogicS _ |- _ =>  symmetry in H
+    | H : Some _ = ilogicS _ |- _ =>  symmetry in H
+    | H : typ2 _ _ = typ2 _ _ |- _ => r_inj H; clear_eq
+    | H : Rty (typ2 _ _) (typ2 _ _) |- _ => r_inj H; clear_eq
+    | H : Rcast option _ (Some _) = Some _ |- _ => apply Rcast_option_inj in H; subst
+    | H1 : baseS ?f = Some (pString ?typ ?s), H2 : funcAs ?f ?t = Some _ |- _ =>
+      assert (t = tyString) by (apply (bf_string_type_eq _ _ H1 H2)); subst;
+      let H := fresh "H" in
+      assert (funcAs f tyString = funcAs (pString typ s) tyString) as H by
+        (apply bf_funcAsOk; assumption); 
+      rewrite H in H2; clear H;
+      unfold funcAs in H2; simpl in H2; rewrite type_cast_refl in H2;
+        [| apply _]
+      
+    | H1 : open_funcS ?f = Some (of_apply_subst ?t), H2 : funcAs ?f ?u = Some _ |- _ =>
+      let v := constr:(typ2 (typ2 (typ2 tyString tyVal) t) (typ2 tySubst (typ2 (typ2 tyString tyVal) t))) in
+      let Heq := fresh "Heq" in assert (u = v) as Heq by (apply (of_apply_subst_type_eq _ _ H1 H2)); r_inj Heq;
+      let H := fresh "H" in pose proof (of_funcAsOk _ H1) as H;
+      rewrite H in H2; clear H;
+      unfold funcAs in H2; simpl in H2; rewrite type_cast_refl in H2;
+        [| apply _]
+      
+    | H1 : open_funcS ?f = Some (of_const ?t), H2 : funcAs ?f ?u = Some _ |- _ =>
+      let v := constr:(typ2 t (typ2 (typ2 tyString tyVal) t)) in
+      let Heq := fresh "Heq" in assert (u = v) as Heq by (apply (of_const_type_eq _ _ H1 H2)); r_inj Heq;
+      let H := fresh "H" in
+      pose proof (of_funcAsOk _ H1) as H;
+      rewrite H in H2; clear H;
+      unfold funcAs in H2; simpl in H2; rewrite type_cast_refl in H2 ;
+        [| apply _]
+        
+    | H1 : open_funcS ?f = Some (of_ap ?t ?u), H2 : funcAs ?f ?v = Some _ |- _ =>
+      let w := constr:(typ2 (typ2 (typ2 tyString tyVal) (typ2 t u)) (typ2 (typ2 (typ2 tyString tyVal) t) (typ2 (typ2 tyString tyVal) u))) in
+      let Heq := fresh "Heq" in assert (v = w) as Heq by (apply (of_ap_type_eq _ _ H1 H2)); r_inj Heq;
+      let H := fresh "H" in
+      pose proof (of_funcAsOk _ H1) as H;
+      rewrite H in H2; clear H;
+      unfold funcAs in H2; simpl in H2; rewrite type_cast_refl in H2 ;
+        [| apply _]
+        
+    | H1 : open_funcS ?f = Some (of_single_subst), H2 : funcAs ?f ?t = Some _ |- _ =>
+      let u := constr:(typ2 (typ2 (typ2 tyString tyVal) tyVal) (typ2 tyString tySubst)) in
+      let Heq := fresh "Heq" in assert (t = u) as Heq
+       by (apply (of_single_subst_type_eq _ _ H1 H2)); r_inj Heq;
+      let H := fresh "H" in
+      pose proof (of_funcAsOk _ H1) as H;
+      rewrite H in H2; clear H;
+      unfold funcAs in H2; simpl in H2; rewrite type_cast_refl in H2 ;
+        [| apply _]
+        
+    | H1 : open_funcS ?f = Some of_stack_get, H2 : funcAs ?f ?u = Some _ |- _ =>
+      let v := constr:(typ2 tyString (typ2 (typ2 tyString tyVal) tyVal)) in
+      let Heq := fresh "Heq" in assert (u = v) as Heq
+       by (apply (of_stack_get_type_eq _ _ H1 H2)); r_inj Heq;
+      let H := fresh "H" in
+      pose proof (of_funcAsOk _ H1) as H;
+      rewrite H in H2; clear H;
+      unfold funcAs in H2; simpl in H2; rewrite type_cast_refl in H2;
+        [| apply _]
+
+    | H1 : bilogicS ?f = Some (bilf_emp ?t), H2 : funcAs ?f ?u = Some _ |- _ =>
+      let Heq := fresh "Heq" in assert (t = u) 
+       by (apply (bilf_emp_type_eq _ _ H1 H2));
+      let H := fresh "H" in
+      pose proof (bilf_funcAsOk _ H1) as H;
+      rewrite H in H2; clear H ;
+      unfold funcAs in H2; simpl in H2; forward; inv_all; subst
+
+    | H1 : bilogicS ?f = Some (bilf_star ?t), H2 : funcAs ?f ?u = Some _ |- _ =>
+      let Heq := fresh "Heq" in assert (u = typ2 t (typ2 t t)) 
+       by (apply (bilf_star_type_eq _ _ H1 H2));
+      let H := fresh "H" in
+      pose proof (bilf_funcAsOk _ H1) as H;
+      rewrite H in H2; clear H ;
+      unfold funcAs in H2; simpl in H2; forward; inv_all; subst
+
+    | H1 : bilogicS ?f = Some (bilf_wand ?t), H2 : funcAs ?f ?u = Some _ |- _ =>
+      let Heq := fresh "Heq" in assert (u = typ2 t (typ2 t t)) 
+       by (apply (bilf_wand_type_eq _ _ H1 H2));
+      let H := fresh "H" in
+      pose proof (bilf_funcAsOk _ H1) as H;
+      rewrite H in H2; clear H ;
+      unfold funcAs in H2; simpl in H2; forward; inv_all; subst
+
+    | H1 : ilogicS ?f = Some (ilf_true ?t), H2 : funcAs ?f ?u = Some _ |- _ =>
+      let Heq := fresh "Heq" in assert (t = u) as Heq 
+       by (apply (ilf_true_type_eq _ _ H1 H2));
+      let H := fresh "H" in
+      pose proof (ilf_funcAsOk _ H1) as H;
+      rewrite H in H2; clear H ;
+      unfold funcAs in H2; simpl in H2; forward; inv_all; subst
+
+    | H1 : ilogicS ?f = Some (ilf_false ?t), H2 : funcAs ?f ?u = Some _ |- _ =>
+      let Heq := fresh "Heq" in assert (t = u) as Heq 
+       by (apply (ilf_false_type_eq _ _ H1 H2));
+      let H := fresh "H" in
+      pose proof (ilf_funcAsOk _ H1) as H;
+      rewrite H in H2; clear H ;
+      unfold funcAs in H2; simpl in H2; forward; inv_all; subst
+
+    | H1 : ilogicS ?f = Some (ilf_and ?t), H2 : funcAs ?f ?u = Some _ |- _ =>
+      let Heq := fresh "Heq" in assert (u = tyArr t (tyArr t t)) as Heq 
+       by (apply (ilf_and_type_eq _ _ H1 H2));
+      let H := fresh "H" in
+      pose proof (ilf_funcAsOk _ H1) as H;
+      rewrite H in H2; clear H ;
+      unfold funcAs in H2; simpl in H2; forward; inv_all; subst
+
+    | H1 : ilogicS ?f = Some (ilf_or ?t), H2 : funcAs ?f ?u = Some _ |- _ =>
+      let Heq := fresh "Heq" in assert (u = tyArr t (tyArr t t)) as Heq 
+       by (apply (ilf_or_type_eq _ _ H1 H2));
+      let H := fresh "H" in
+      pose proof (ilf_funcAsOk _ H1) as H;
+      rewrite H in H2; clear H ;
+      unfold funcAs in H2; simpl in H2; forward; inv_all; subst
+
+    | H1 : ilogicS ?f = Some (ilf_impl ?t), H2 : funcAs ?f ?u = Some _ |- _ =>
+      let Heq := fresh "Heq" in assert (u = tyArr t (tyArr t t)) as Heq 
+       by (apply (ilf_impl_type_eq _ _ H1 H2));
+      let H := fresh "H" in
+      pose proof (ilf_funcAsOk _ H1) as H;
+      rewrite H in H2; clear H ;
+      unfold funcAs in H2; simpl in H2; forward; inv_all; subst
+  end.
+
 
   Lemma substTac_ok : partial_reducer_ok (substTac nil).
   Proof.
@@ -216,7 +369,24 @@ Require Import FunctionalExtensionality.
     autorewrite with exprD_rw in H0; simpl in H0; forward; inv_all; subst.
     autorewrite with exprD_rw in H2; simpl in H2; forward; inv_all; subst.
     
-    symmetry in Heqo.
+    repeat forward_step.
+    repeat rewrite Rcast_id.
+    (*
+    forward_step.
+    match goal with 
+        | H1 : open_funcS ?f = Some (of_apply_subst ?t), H2 : funcAs ?f ?u = Some _ |- _ =>
+      let v := constr:(typ2 (typ2 (typ2 tyString tyVal) t) (typ2 tySubst (typ2 (typ2 tyString tyVal) t))) in
+      let Heq := fresh "Heq" in assert (u = v) as Heq by (apply (of_apply_subst_type_eq _ _ H1 H2)); r_inj Heq;
+      let H := fresh "H" in pose proof (of_funcAsOk _ H1) as H ;
+      rewrite H in H2; clear H;
+      unfold funcAs in H2; simpl in H2; rewrite type_cast_refl in H2;
+        [| apply _]
+    end.
+    forward_step.
+    subst.
+    forward_step.
+    r_inj H4.
+    
     pose proof (typeof_funcAs _ _ H2).
     pose proof (OpenFunc_typeOk _ Heqo).
     rewrite H4 in H5. simpl in H5.
@@ -226,947 +396,224 @@ Require Import FunctionalExtensionality.
     unfold Rty in *.
     subst; inv_all; subst.
     clear H6 H12 H11 H5 H8 H10 H9 H4.
-    induction e using expr_strong_ind;
-    try (solve [simpl; eexists; split; [eapply mkApplySubst_sound; eassumption|reflexivity]]).
-    + (* True, False, and Emp *)
+			  forward_step.
+			  clear H7 H5 H8 H4 H10 H9 H11. *)
+    clear Heqo.
+	generalize dependent t0.
+    induction e using expr_strong_ind; intros;
+    try (solve [simpl; eexists; split; [eapply mkApplySubst_sound; eassumption|reflexivity]]). {
+      (* True, False, and Emp *)
       autorewrite with exprD_rw in H3; simpl in H3; forward; inv_all; subst.
 	  simpl; remember (ilogicS i) as o; destruct o; [destruct i0|];
 	  try (solve [simpl; eexists; split; [eapply mkApplySubst_sound; try eassumption; autorewrite with exprD_rw; simpl; forward; inv_all; subst; reflexivity|reflexivity]]);
 	  [| | (remember (bilogicS i) as o; destruct o; [destruct b|])]; 
 	  try (solve [simpl; eexists; split; [eapply mkApplySubst_sound; try eassumption; autorewrite with exprD_rw; simpl; forward; inv_all; subst; reflexivity|reflexivity]]).
-	  * admit.
-	  * admit.
-	  * eexists; split; [eapply mkEmp_sound; [symmetry; eassumption | eassumption]|].
-	    intros. simpl.
-
-  	    autorewrite with exprD_rw in H0; simpl in *.
-  	    clear Heqo0.
-  	    
-
-        pose proof (of_funcAsOk).
-        specialize (H4 _ _ Heqo).
-        rewrite H4 in H2.
-        unfold funcAs in H2. simpl in H2. rewrite type_cast_refl in H2; [|apply _]. unfold Rrefl in H2.
-        apply Rcast_eq_refl in H2. inversion H2; subst; clear H2.
-        unfold fun_to_typ3.
-
-        rewrite exprT_App_wrap.
-        rewrite exprT_App_wrap.
-
-        Require Import BILogic.
-        assert (BILOperators (typD t0)) by admit.
- 
-        unfold fun_to_typ, typ_to_fun, id.
-        unfold eq_rect_r, eq_rect, eq_rec.
-        generalize (typ2_cast tyString tyVal).
-        generalize (typ2_cast (typ2 tyString tyVal) t0).
-        clear -X0.
-        generalize dependent (typ2 tyString tyVal); intro.
-        generalize dependent (typ2 t t0); intro.
-        generalize dependent (typ2 t t0); intro.
-        generalize dependent (typD t1).
-        generalize dependent (typD t).
-        intros; subst; simpl.
-
-        Require Import BILInsts.
-        Existing Instance BILFun_Ops.
-        Require Import ILInsts.
-        Existing Instance ILFun_Ops.
-        assert (t2 = empSP) by admit. subst.
-        reflexivity.
-      + autorewrite with exprD_rw in H3; simpl in H3; forward; inv_all; subst.
-        simpl.
-        destruct e1; autorewrite with exprD_rw in H5; simpl in H5; forward; inv_all; subst;
+	  { (* True *)
+	    repeat forward_step.
+	    unfold applySubstD, fun_to_typ3; repeat rewrite exprT_App_wrap.
+	    eexists; split; [eapply mkTrue_sound; eassumption|]; intros.
+	    admit.
+	  } { (* False *) 
+	    repeat forward_step.
+	    unfold applySubstD, fun_to_typ3; repeat rewrite exprT_App_wrap.
+	    eexists; split; [eapply mkFalse_sound; eassumption|]; intros.
+	    admit.
+	  } { (* Emp *)	    
+	    repeat forward_step.
+	    unfold applySubstD, fun_to_typ3; repeat rewrite exprT_App_wrap.
+	    eexists; split; [eapply mkEmp_sound; eassumption|]; intros.
+	    admit.
+	 }
+   } {
+     autorewrite with exprD_rw in H3; simpl in H3; forward; inv_all; subst; simpl.
+     destruct e1; autorewrite with exprD_rw in H4; simpl in H4; forward; inv_all; subst;
+     try (solve [simpl; eexists; split; [eapply mkApplySubst_sound; try eassumption; repeat (autorewrite with exprD_rw; simpl; forward; inv_all; subst); reflexivity|reflexivity]]).
+     remember (open_funcS f0); destruct o; [destruct o|];
+     try (solve [simpl; eexists; split; [eapply mkApplySubst_sound; try eassumption; repeat (autorewrite with exprD_rw; simpl; forward; inv_all; subst); reflexivity|reflexivity]]).
+     { (* const *)
+       repeat forward_step.
+       rewrite Rcast_id.
+       eexists; split; [eapply mkConst_sound; eassumption|]; intros.
+       unfold applySubstD, constD, fun_to_typ3; repeat rewrite exprT_App_wrap.
+       admit.
+     } { (* applySubst *)
+		destruct e3; autorewrite with exprD_rw in H5; simpl in H5; forward; inv_all; subst;
+        autorewrite with exprD_rw in H3; simpl in H3; forward; inv_all; subst;
+        try (solve [simpl; eexists; split; [eapply mkApplySubst_sound; try eassumption; 
+          repeat (autorewrite with exprD_rw; simpl; forward; inv_all; subst); try (rewrite H11 in H9; inv_all; subst; forward; inv_all; subst); reflexivity|reflexivity]]).
+        remember (baseS f1); destruct o; [destruct b|];
+          try (solve [eexists; split; [eapply mkApplySubst_sound; try eassumption|reflexivity];
+              repeat (autorewrite with exprD_rw; simpl; forward; inv_all; subst); reflexivity]).
+		destruct e0; simpl;
         try (solve [simpl; eexists; split; [eapply mkApplySubst_sound; try eassumption; repeat (autorewrite with exprD_rw; simpl; forward; inv_all; subst); reflexivity|reflexivity]]).
-        remember (open_funcS f0); destruct o; [destruct o|];
+		destruct e0_1; simpl;
         try (solve [simpl; eexists; split; [eapply mkApplySubst_sound; try eassumption; repeat (autorewrite with exprD_rw; simpl; forward; inv_all; subst); reflexivity|reflexivity]]).
-        
-        * 
-        
-			  Lemma Rcast_option_inj (t u : typ) r (a : typD t) (b : typD u)
-			    (H : Rcast option r (Some a) = Some b) :
-			    b = Rcast id r a.
-			  Proof.
-			    clear -H.
-			    unfold Rcast, Relim, Rsym, eq_sym in *.
-			    destruct r; inv_all; subst. reflexivity.
-			  Qed.
+		destruct e0_1_1; simpl;
+        try (solve [simpl; eexists; split; [eapply mkApplySubst_sound; try eassumption; repeat (autorewrite with exprD_rw; simpl; forward; inv_all; subst); reflexivity|reflexivity]]).
+		remember (open_funcS f2). destruct o;
+        try (solve [simpl; eexists; split; [eapply mkApplySubst_sound; try eassumption; repeat (autorewrite with exprD_rw; simpl; forward; inv_all; subst); reflexivity|reflexivity]]).
+		destruct o; simpl;
+        try (solve [simpl; eexists; split; [eapply mkApplySubst_sound; try eassumption; repeat (autorewrite with exprD_rw; simpl; forward; inv_all; subst); reflexivity|reflexivity]]).
+		destruct e0_2; simpl;
+        try (solve [simpl; eexists; split; [eapply mkApplySubst_sound; try eassumption; repeat (autorewrite with exprD_rw; simpl; forward; inv_all; subst); reflexivity|reflexivity]]).
+		remember (baseS f3); destruct o; [destruct b|];
+        try (solve [simpl; eexists; split; [eapply mkApplySubst_sound; try eassumption; repeat (autorewrite with exprD_rw; simpl; forward; inv_all; subst); reflexivity|reflexivity]]).
+		unfold applySingleSubst.
+		clear H0.
 
-        Ltac r_inj_aux H :=
-            first [
-              let H1 := fresh "H" in let H2 := fresh "H" in
-                apply typ2_inj in H as [H1 H2]; [unfold Rty in H1, H2; r_inj_aux H1; r_inj_aux H2 | apply _] |
-              repeat subst].
+		autorewrite with exprD_rw in H1; simpl in H1; forward; inv_all; subst.
+		autorewrite with exprD_rw in H6; simpl in H6; forward; inv_all; subst.
+		autorewrite with exprD_rw in H1; simpl in H1; forward; inv_all; subst.
+		autorewrite with exprD_rw in H7; simpl in H7; forward; inv_all; subst.
+		
+		consider (s ?[ eq ] s0). {
+		  intros; subst; repeat forward_step.
+		  repeat rewrite Rcast_id.
+		  unfold applySubstD, stack_getD, singleSubstD, fun_to_typ3, fun_to_typ2.
+		  repeat rewrite exprT_App_wrap.
+		  eexists; split; [eassumption|].
+		  intros. 
+		  admit.
+		} {
+		  intros.
+		  repeat (autorewrite with exprD_rw; simpl; forward; inv_all; subst).
+		  eexists; split; [reflexivity|].
+		  intros; repeat forward_step.
+		  unfold applySubstD, stack_getD, singleSubstD, fun_to_typ3, fun_to_typ2.
+		  repeat rewrite exprT_App_wrap.
+		  repeat rewrite Rcast_id.
+		  repeat rewrite exprT_App_wrap.
+		  admit.
+	   }
+	 } { (* embed *)
+ 	   remember (embedS f0); destruct o; [destruct e|]; [|
+         simpl; eexists; split; [eapply mkApplySubst_sound; try eassumption; repeat (autorewrite with exprD_rw; simpl; forward; inv_all; subst); reflexivity|reflexivity]
+	   ].
+  	   admit. (* Need to check if one logic is embedded in the other *)
+  	 } {
+       destruct e1_1; simpl; autorewrite with exprD_rw in H6; simpl in H6; forward; inv_all; subst;
+       try (solve [simpl; eexists; split; [eapply mkApplySubst_sound; try eassumption; repeat (autorewrite with exprD_rw; simpl; forward; inv_all; subst); reflexivity|reflexivity]]).
+	   remember (ilogicS f0); destruct o; [destruct i|];
+       try (solve [simpl; eexists; split; [eapply mkApplySubst_sound; try eassumption; repeat (autorewrite with exprD_rw; simpl; forward; inv_all; subst); reflexivity|reflexivity]]).
+	   {
+	    assert (TransitiveClosure.leftTrans (expr_acc (func := func)) e1_2 (App (App (Inj f0) e1_2) e3))
+	      by (eapply TransitiveClosure.LTStep; [apply acc_App_r | constructor; eapply acc_App_l]).
+	    assert (TransitiveClosure.leftTrans (expr_acc (func := func)) e3 (App (App (Inj f0) e1_2) e3))
+	      by (constructor; apply acc_App_r).
+	    repeat forward_step.
 
-        Ltac r_inj :=
-          match goal with
-            | H : typ2 _ _ = typ2 _ _ |- _ => r_inj_aux H
-          end.
-Check of_funcAsOk.
-			Ltac forward_step :=
-			  match goal with 
-			    | H : Some _ = baseS _ |- _ =>  symmetry in H
-			    | H : Some _ = open_funcS _ |- _ =>  symmetry in H
-			    | H1 : baseS ?f = Some (pString ?typ ?s), H2 : funcAs ?f ?t = Some _ |- _ =>
-			      assert (t = tyString) by (apply (bf_string_type_eq _ _ H1 H2)); subst;
-			      let H := fresh "H" in
-			      assert (funcAs f tyString = funcAs (pString typ s) tyString) as H by
-			        (apply bf_funcAsOk; assumption); 
-			      rewrite H in H2; clear H;
-			      unfold funcAs in H2; simpl in H2; rewrite type_cast_refl in H2;
-			        [apply Rcast_option_inj in H2; subst | apply _]
-			      
-			    | H1 : open_funcS ?f = Some (of_apply_subst ?t), H2 : funcAs ?f ?u = Some _ |- _ =>
-			      let v := constr:(typ2 (typ2 (typ2 tyString tyVal) t) (typ2 tySubst (typ2 (typ2 tyString tyVal) t))) in
-			      assert (u = v) by (apply (of_apply_subst_type_eq _ _ H1 H2)); r_inj;
-			      let H := fresh "H" in pose proof (of_funcAsOk _ H1) as H;
-			      rewrite H in H2; clear H;
-			      unfold funcAs in H2; simpl in H2; rewrite type_cast_refl in H2;
-			        [apply Rcast_option_inj in H2; subst | apply _]
-			      
-			    | H1 : open_funcS ?f = Some (of_const ?t), H2 : funcAs ?f ?u = Some _ |- _ =>
-			      let v := constr:(typ2 t (typ2 (typ2 tyString tyVal) t)) in
-			      assert (u = v) 
-			       by (apply (of_const_type_eq _ _ H1 H2)); r_inj;
-			      let H := fresh "H" in
-			      pose proof (of_funcAsOk _ H1) as H;
-			      rewrite H in H2; clear H;
-			      unfold funcAs in H2; simpl in H2; rewrite type_cast_refl in H2 ;
-			        [apply Rcast_option_inj in H2; subst | apply _]
-			        
-			  end.
-			  
-        eexists; split.
-        eapply mkConst_sound. symmetry. eassumption. eassumption.
-        forward_step.
-        forward_step.
-        forward_step.
-        eexists; split.
-        eapply mkConst_sound. eassumption. eassumption.
-        r_inj.
-        Check typ2_inj.
-        unfold tyArr in *.
-          
-        r_inj.
-        
-        
-        
-        clear H7.
-        clear H11.
-        subst. clear H13.
-        subst.
-        inv_all. subst.
-        clear H14.
-        repeat r_inj.
-        unfold Rty in H8, H9.
-        r_inj.
-        r_inj.
-        r_inj.
-        unfold tyArr.
-        eapply of_apply_subst_type_eq. eassumption. eassumption.
-        reflexivity.
-        symmetry in Heqo0. 
-          assert (t2 = t) by (eapply const_type1; eassumption); subst.
-          assert (t = t0) by (eapply const_type2; eassumption); subst.
-          eexists; split; [eapply mkConst_sound; try eassumption|].
-          intros.
-          
-          pose proof (of_funcAsOk).
-          specialize (H7 _ _ Heqo).
-          rewrite H7 in H2.
-          unfold funcAs in H2. simpl in H2. rewrite type_cast_refl in H2; [|apply _]. unfold Rrefl in H2.
-          apply Rcast_eq_refl in H2. inversion H2; subst; clear H2.
+	    destruct (H0 _ H8 _ H4 _ H7) as [? [? ?]].
+	    destruct (H0 _ H9 _ H3 _ H5) as [? [? ?]].
+	    clear H0.
+		eexists; split; [eapply mkAnd_sound; eassumption|]; intros.
+		specialize (H12 _ _ X); specialize (H14 _ _ X).
 
-          pose proof (of_funcAsOk).
-          specialize (H2 _ _ Heqo0).
-          rewrite H2 in H5.
-          unfold funcAs in H5. simpl in H5. rewrite type_cast_refl in H5; [|apply _]. unfold Rrefl in H5.
-          apply Rcast_eq_refl in H5. inversion H5; subst; clear H5.
-          unfold fun2_wrap, fun_to_typ3.
+		unfold applySubstD, andD, fun_to_typ2, fun_to_typ3; repeat rewrite exprT_App_wrap. 
+		rewrite <- H12, <- H14.
+		unfold applySubstD, fun_to_typ3; repeat rewrite exprT_App_wrap.
+		admit.
+      } {
+	    assert (TransitiveClosure.leftTrans (expr_acc (func := func)) e1_2 (App (App (Inj f0) e1_2) e3))
+	      by (eapply TransitiveClosure.LTStep; [apply acc_App_r | constructor; eapply acc_App_l]).
+	    assert (TransitiveClosure.leftTrans (expr_acc (func := func)) e3 (App (App (Inj f0) e1_2) e3))
+	      by (constructor; apply acc_App_r).
+	    repeat forward_step.
 
-          rewrite exprT_App_wrap.
-          rewrite exprT_App_wrap.
-          rewrite exprT_App_wrap.
-          
-          unfold fun_to_typ, typ_to_fun, id, fun1_wrap.
-          unfold eq_rect_r, eq_rect, eq_rec.
-          generalize (typ2_cast tyString tyVal).
-          generalize (typ2_cast (typ2 tyString tyVal) t0).
-          clear.
-          generalize dependent (typ2 tyString tyVal); intro.
-          generalize dependent (typ2 t t0); intro.
-          generalize dependent (typ2 t t0); intro.
-          generalize dependent (typD t1).
-          generalize dependent (typD t).
-          generalize dependent (typD t0).
-          intros; subst; simpl.
-		  reflexivity.
-		* destruct e3; autorewrite with exprD_rw in H6; simpl in H6; forward; inv_all; subst;
-          autorewrite with exprD_rw in H3; simpl in H3; forward; inv_all; subst;
+	    destruct (H0 _ H8 _ H4 _ H7) as [? [? ?]].
+	    destruct (H0 _ H9 _ H3 _ H5) as [? [? ?]].
+	    clear H0.
+		eexists; split; [eapply mkOr_sound; eassumption|]; intros.
+		specialize (H12 _ _ X); specialize (H14 _ _ X).
+
+		unfold applySubstD, orD, fun_to_typ2, fun_to_typ3; repeat rewrite exprT_App_wrap. 
+		rewrite <- H12, <- H14.
+		unfold applySubstD, fun_to_typ3; repeat rewrite exprT_App_wrap.
+		admit.
+      } {
+	    assert (TransitiveClosure.leftTrans (expr_acc (func := func)) e1_2 (App (App (Inj f0) e1_2) e3))
+	      by (eapply TransitiveClosure.LTStep; [apply acc_App_r | constructor; eapply acc_App_l]).
+	    assert (TransitiveClosure.leftTrans (expr_acc (func := func)) e3 (App (App (Inj f0) e1_2) e3))
+	      by (constructor; apply acc_App_r).
+	    repeat forward_step.
+
+	    destruct (H0 _ H8 _ H4 _ H7) as [? [? ?]].
+	    destruct (H0 _ H9 _ H3 _ H5) as [? [? ?]].
+	    clear H0.
+		eexists; split; [eapply mkImpl_sound; eassumption|]; intros.
+		specialize (H12 _ _ X); specialize (H14 _ _ X).
+
+		unfold applySubstD, implD, fun_to_typ2, fun_to_typ3; repeat rewrite exprT_App_wrap. 
+		rewrite <- H12, <- H14.
+		unfold applySubstD, fun_to_typ3; repeat rewrite exprT_App_wrap.
+		admit.
+     } {
+       remember (open_funcS f0); destruct o; [destruct o;
+         try (solve [simpl; eexists; split; [eapply mkApplySubst_sound; try eassumption; repeat (autorewrite with exprD_rw; simpl; forward; inv_all; subst); reflexivity|reflexivity]])
+       |].
+       {
+	     assert (TransitiveClosure.leftTrans (expr_acc (func := func)) e1_2 (App (App (Inj f0) e1_2) e3))
+	       by (eapply TransitiveClosure.LTStep; [apply acc_App_r | constructor; eapply acc_App_l]).
+	     assert (TransitiveClosure.leftTrans (expr_acc (func := func)) e3 (App (App (Inj f0) e1_2) e3))
+	       by (constructor; apply acc_App_r).
+	     repeat forward_step.
+	     
+	    destruct (H0 _ H8 _ H4 _ H7) as [? [? ?]].
+	    destruct (H0 _ H9 _ H3 _ H5) as [? [? ?]].
+	    clear H0.
+		eexists; split; [eapply mkAp_sound; eassumption|]; intros.
+		specialize (H10 _ _ X); specialize (H14 _ _ X).
+	    rewrite Rcast_id.
+		unfold applySubstD, apD, fun_to_typ2, fun_to_typ3; repeat rewrite exprT_App_wrap. 
+		rewrite <- H10, <- H14.
+		unfold applySubstD, fun_to_typ3; repeat rewrite exprT_App_wrap.
+		admit.
+      } {
+        remember (bilogicS f0); destruct o; [destruct b|];
           try (solve [simpl; eexists; split; [eapply mkApplySubst_sound; try eassumption; repeat (autorewrite with exprD_rw; simpl; forward; inv_all; subst); reflexivity|reflexivity]]).
-          { remember (baseS f1); destruct o; [destruct b|];
-              try (solve [eexists; split; [eapply mkApplySubst_sound; try eassumption|reflexivity];
-                repeat (autorewrite with exprD_rw; simpl; forward; inv_all; subst); reflexivity]).
+	    { (* Star *) 
+	      assert (TransitiveClosure.leftTrans (expr_acc (func := func)) e1_2 (App (App (Inj f0) e1_2) e3))
+	        by (eapply TransitiveClosure.LTStep; [apply acc_App_r | constructor; eapply acc_App_l]).
+	      assert (TransitiveClosure.leftTrans (expr_acc (func := func)) e3 (App (App (Inj f0) e1_2) e3))
+	        by (constructor; apply acc_App_r).
+	      repeat forward_step.
+	     
+	      destruct (H0 _ H8 _ H4 _ H7) as [? [? ?]].
+	      destruct (H0 _ H9 _ H3 _ H5) as [? [? ?]].
+	      clear H0.
+		  eexists; split; [eapply mkStar_sound; eassumption|]; intros.
+		  specialize (H12 _ _ X); specialize (H14 _ _ X).
 
-            pose proof (of_funcAsOk).
-            symmetry in Heqo0.
-            pose proof (stack_get_type _ _ _ _ _ Heqo0 H5) as [? [? [? ?]]]; subst.
-			destruct e0; simpl;
-            try (solve [simpl; eexists; split; [eapply mkApplySubst_sound; try eassumption; repeat (autorewrite with exprD_rw; simpl; forward; inv_all; subst); reflexivity|reflexivity]]).
-			destruct e0_1; simpl;
-            try (solve [simpl; eexists; split; [eapply mkApplySubst_sound; try eassumption; repeat (autorewrite with exprD_rw; simpl; forward; inv_all; subst); reflexivity|reflexivity]]).
-			destruct e0_1_1; simpl;
-            try (solve [simpl; eexists; split; [eapply mkApplySubst_sound; try eassumption; repeat (autorewrite with exprD_rw; simpl; forward; inv_all; subst); reflexivity|reflexivity]]).
-			remember (open_funcS f2). destruct o;
-            try (solve [simpl; eexists; split; [eapply mkApplySubst_sound; try eassumption; repeat (autorewrite with exprD_rw; simpl; forward; inv_all; subst); reflexivity|reflexivity]]).
-			destruct e0_2; simpl;
-            try (solve [simpl; eexists; split; [eapply mkApplySubst_sound; try eassumption; repeat (autorewrite with exprD_rw; simpl; forward; inv_all; subst); reflexivity|reflexivity]]).
-			remember (baseS f3); destruct o0; [destruct b|];
-            try (solve [simpl; eexists; split; [eapply mkApplySubst_sound; try eassumption; repeat (autorewrite with exprD_rw; simpl; forward; inv_all; subst); reflexivity|reflexivity]]).
-			unfold applySingleSubst.
-			clear H4.
-			
-			autorewrite with exprD_rw in H1; simpl in H1; forward; inv_all; subst.
-			autorewrite with exprD_rw in H8; simpl in H8; forward; inv_all; subst.
-			autorewrite with exprD_rw in H4; simpl in H4; forward; inv_all; subst.
-			autorewrite with exprD_rw in H11; simpl in H11; forward; inv_all; subst.
-			
-			symmetry in Heqo3.
-			Check (bf_string_type_eq _ _ Heqo3).
-			Check bf_funcAsOk.
-			Check pString.
-			  
+		  unfold applySubstD, starD, fun_to_typ2, fun_to_typ3; repeat rewrite exprT_App_wrap. 
+	      rewrite <- H12, <- H14.
+		  unfold applySubstD, fun_to_typ3; repeat rewrite exprT_App_wrap.
+		  admit.
+	    } { (* Wand *) 
+	      assert (TransitiveClosure.leftTrans (expr_acc (func := func)) e1_2 (App (App (Inj f0) e1_2) e3))
+	        by (eapply TransitiveClosure.LTStep; [apply acc_App_r | constructor; eapply acc_App_l]).
+	      assert (TransitiveClosure.leftTrans (expr_acc (func := func)) e3 (App (App (Inj f0) e1_2) e3))
+	        by (constructor; apply acc_App_r).
+	      repeat forward_step.
+	     
+	      destruct (H0 _ H8 _ H4 _ H7) as [? [? ?]].
+	      destruct (H0 _ H9 _ H3 _ H5) as [? [? ?]].
+	      clear H0.
+		  eexists; split; [eapply mkWand_sound; eassumption|]; intros.
+		  specialize (H12 _ _ X); specialize (H14 _ _ X).
 
-			  forward_step.
-			  forward_step.
-			  forward_step.
-			  forward_step.
-			  clear Heqo3.
-			  symmetry in Heqo1.
-			  forward_step.
-			      apply Rcast_option_inj in H8; subst.
-			  SearchAbout Rcast option.
-			  Check Rcast.
-			  
-			  unfold Rcast, Relim, Rrefl, Rsym in H8.
-			  assert (typD tyString = String.string). admit. subst.
-			  generalize dependent t0. rewrite H13.
-			  assert (t0 : typD tyString).
-			  generalize (typD tyString).
-			  generalize dependent t0.
-			  Check (@tyString typ _).
-			  replace (typD (@tyString typ BT)) with String.string.
-			  rewrite btString in t0.
-			  unfold Rcast, Relim, Rsym, eq_rect_r, eq_rect, eq_sym in H8.
-			  simpl in H8.
-			  unfold id in H8.
-			  Check btString.
-			  destruct btString.
-			  rewrite btString in H8.
-			  inversion H8. subst.
-			  rewrite 
-			  unfold btString in H8. simpl in H8.
-			  inversion H8.
-			  apply bf_funcAsOk; eassumption.
-			  assert (t0 = tyString) by (apply (bf_string_type_eq _ _ Heqo3 H8)).
-			  Check (bf_string_type_eq _ _ Heqo3 H8).
-forward_step.
-			pose proof (bf_funcAsOk); symmetry in Heqo3.
-			specialize (H13 _ _ Heqo3).
-			rewrite H13 in H8.
-			unfold funcAs in H8.
-			simpl in H8.
-			
-			
-			pose proof of_funcAsOk.
-			
-			Check baseS.
-			Check open_funcS.
-			Check @bf_funcAsOk.
-			 specialize (H13 _ _ Heqo3).
-			
-			Check nat_sound.
-			
-			consider (s ?[ eq ] s0); intros.
-			Focus 2.
-			simpl; eexists; split.
-			repeat (autorewrite with exprD_rw; simpl; forward; inv_all; subst). reflexivity.
-			reflexivity.
-            try (solve [simpl; eexists; split; [eapply mkApplySubst_sound; try eassumption; repeat (autorewrite with exprD_rw; simpl; forward; inv_all; subst); reflexivity|reflexivity]]).
-
-			unfold applySubst.
-			
-            specialize (H7 _ _ Heqo0).
-            
-            rewrite H7 in H5.
-            unfold funcAs in H5. simpl in H5. rewrite type_cast_refl in H5; [|apply _]. unfold Rrefl in H5.
-            apply Rcast_eq_refl in H5. inversion H5; subst; clear H5.
-          
-              eexists; split; [eapply mkApplySubst_sound;try eassumption|].
-        Focus 2.
-        eexists; split; [eapply mkApplySubst_sound; try eassumption|reflexivity].
-        autorewrite with exprD_rw in H0; simpl in H0; forward; inv_all; subst.
-        repeat (autorewrite with exprD_rw; simpl; forward; inv_all; subst).
-        red_exprD.
-        eexists; split; [eapply mkApplySubst_sound; try eassumption;
-          repeat (autorewrite with exprD_rw; simpl; forward; inv_all; subst)|reflexivity].
-        simpl.
-        
-        eexists; split; [eapply mkApplySubst_sound; try eassumption; autorewrite with exprD_rw; simpl; forward; inv_all; subst;
-          autorewrite with exprD_rw; simpl; forward; inv_all; subst;
-          autorewrite with exprD_rw in H5; simpl in H5; forward |reflexivity].
-          autorewrite with exprD_rw in H5; simpl in H5; forward.
-        try (solve [simpl; eexists; split; [eapply mkApplySubst_sound; try eassumption; autorewrite with exprD_rw; simpl; forward; inv_all; subst; reflexivity|reflexivity]]).
-        
-        unfold apply_subst. simpl.
-        reflexivity.
-        apply functional_extensionality.
-        intros x.
-      reflexivity. apply _.
-      unfold apply_subst.
-      
-      unfold apply_subst. simpl.
-      f_equal.
-          cut (exprT tus tvs (typD (typ2 (typ2 tyString tyVal) t0))).
-          intro X. exists X. split. admit.
-          intros.
-          unfold fun_to_typ, typ_to_fun, id.
-          unfold eq_rect_r, eq_rect, eq_rec.
-          generalize (typ2_cast tyString tyVal).
-          generalize (typ2_cast (typ2 tyString tyVal) t0).
-          { clear.
-            generalize dependent (typ2 tyString tyVal).
-            intro.
-            generalize dependent (typ2 t t0).
-            intro.
-            generalize dependent (typD t1).
-            generalize dependent (typD t).
-            intros; subst. simpl.
-            simpl.
-            unfold stSubst.
-            simpl.
-            pose proof (of_funcAsOk).
-      specialize (H4 _ _ Heqo).
-      rewrite H4 in H2.
-      unfold funcAs in H2. simpl in H2. rewrite type_cast_refl in H2. unfold Rrefl in H2.
-      apply Rcast_eq_refl in H2. inversion H2; subst; clear H2.
-      unfold fun3_wrap.
-      unfold fun2_wrap.
-      unfold fun_to_typ3.
-      rewrite exprT_App_wrap.
-      rewrite exprT_App_wrap.
-      Locate fun_to_typ.
-      unfold eq_rect.
-      symmetry in Heqo1.
-      eexists. split.
-      eapply mkEmp_sound; [eapply Heqo1|eapply H3].
-      intros.
-      pose proof (bilf_funcAsOk i Heqo1). simpl in H4.
-      rewrite H2 in H3.
-      unfold funcAs in H3; simpl in H3; forward.
-      unfold Rty in r.
-      subst.
-      apply Rcast_eq_refl in H6. inv_all; subst.
-      Check fun1D.
-      unfold fun1_wrap, fun1D, eq_rect_r, eq_rect, eq_sym.
-      remember (typ2_cast (typ2 tyString tyVal) t0).
-      inversion e; subst.
-      remember (typ2_cast (typ2 tyString tyVal) t0).
-      generalize dependent e.
-      rewrite H7.
-      rewrite H7 in e.
-      do 2 rewrite typ2_cast in H7.
-      unfold Fun in H7.
-      remember (typ2_cast (typ2 tyString tyVal) t0).
-      rewrite (UIP_refl H7).
-      assert (forall (x:Type) (p:x = x), p = eq_refl x) by admit.
-      remember (typ2_cast (typ2 tyString tyVal) t0).
-      unfold Fun in e.
-      subst.
-      remember (typ2_cast (typ2 tyString tyVal) t0).
-      unfold id.
-      remember (typ2_cast tyString tyVal).
-      assert(forall (x y:Type) (p1 p2:x = y), p1 = p2) by admit.
-      pose proof e1 as e3.
-      specialize (H7 _ _ e1 e3).
-      assert (typD (typ2 tyString tyVal) = Fun (typD tyString) (typD tyVal)) by (apply typ2_cast).
-      generalize dependent e3.
-      rewrite H8.
-      subst.
-      Check typ2_cast.
-      rewrite (@typ2_cast typ RType_typ Fun _ tyString tyVal).
-      generalize dependent (fun y : typD (typ2 tyString tyVal) =>
-    apply_subst
-      (fun x : stack (typD tyString) (typD tyVal) =>
-       match e in (_ = y0) return (id y0) with
-       | eq_refl => BILogic.empSP
-       end
-         match
-           match
-             typ2_cast tyString tyVal in (_ = y0)
-             return (y0 = typD (typ2 tyString tyVal))
-           with
-           | eq_refl => eq_refl
-           end in (_ = y0) return (id y0)
-         with
-         | eq_refl => x
-         end)
-      match stSubst in (_ = y0) return (id y0) with
-      | eq_refl => e2 us vs
-      end).
-      
-      
-      assert (typD (typ2 (typ2 tyString tyVal) t0) = Fun (typD (typ2 tyString tyVal)) (typD t0)) by (apply typ2_cast).
-      progress eapply eq_ind_r with (typD (typ2 (typ2 tyString tyVal) t0)); [|symmetry; eapply H7].
-      subst.
-      assert (typD (typ2 tyString tyVal) = Fun (typD tyString) (typD tyVal)) by (apply typ2_cast).
-      subst.
-      apply typ2_cast.
-      SearchAbout typD typ2.
-      generalize dependent e.
-      Check typ2_cast.
-      
-      rewrite (@typ2_cast typ RType_typ Fun _ tyString tyVal).
- specialize (H6 _ Heqe).
-      SearchAbout typ2_cast.
-      Check typ2_cast.
-      generalize dependent (e2 us vs). intros.
-      generalize dependent (BILogic.empSP). intros.
-      generalize dependent (typ2_cast tyString tyVal). intros.
-      generalize dependent (typ2_cast (typ2 tyString tyVal)).
-      intros.
-      destruct stSubst.
-      destruct e.
-      destruct e.
-      destruct (typ2_cast tyString tyVal).
-      
-      destruct (typ2_cast (typ2 tyString tyVal) t0).
-      Lemma blurb f : (fun x => (fun1D Typ2_tyArr f) (fun1_wrap Typ2_tyArr x)) = fun1D _ f.
-      
-      unfold fun1_wrap.
-      unfold eq_rect_r, eq_rect, eq_sym. simpl. forward.
-      specialize (H5 (typ2 (typ2 tyString tyVal) t0)).
-      rewrite H5 in H3. simpl. inv_all; subst. simpl in H3.
-      Check bilf_funcAsOk.
-      simpl in H3.
-      unfold funcAs in H3. simpl in H3. forward. inv_all; subst.
-     destruct r; subst. 
-     
-     
-      Lemma Rcast_option (t u : typ) (r : Rty t u) (a : typD t) (b : typD u) (H : Rcast option r (Some a) = Some b) :
-        Rcast (fun T => T) r a = b.
-      Proof.
-        unfold Rcast, Relim, Rsym in *.
-        destruct r; unfold eq_sym in *.
-        inversion H; subst; reflexivity.
-      Qed.
-      
-      apply Rcast_eq_refl in H7.
-      inversion H7; subst; clear H7.
-      
-      
-      
-      apply Rcast_option in H7.
-      unfold Rcast, Relim, Rsym, eq_sym in H7.
-      destruct r. subst.
-      simpl in *.
-      SearchAbout Rcast.
-      Check Rcast.
-      Print Rcast.
-      unfold Rcast, Relim, Rsym, eq_sym in H7.
-      forward.
-      unfold Rty in r.
-      SearchAbout type_cast.
-      unfold type_cast in H6. simpl in H6.
-      rewrite r in H7.
-      pose proof (bilf_fStarOk logic0) as HfuncOk.
-      rewrite H4 in *.
-      specialize
-      Lemma test tus tvs (t u : typ) (f : exprT tus tvs (typD (typ2 t u))) g us vs : exists x, exprT_App f g us vs = x.
-      Proof.
-        unfold exprT_App.
-        simpl.
-        unfold eq_sym.
-        generalize dependent ( fun (f0 : exprT tus tvs (typD t -> typD u))
-        (x0 : exprT tus tvs (typD t)) (us0 : HList.hlist typD tus)
-        (vs0 : HList.hlist typD tvs) => f0 us0 vs0 (x0 us0 vs0)). intros.
-        SearchAbout typ2_cast.
-        unfold typ2_cast. simpl.
-        destruct (typ2_cast t u).
-      unfold exprT_App.
-      simpl.
-      SearchAbout exprT_App.
-      unfold exprT_App, eq_sym.
-      destruct (typ2_cast (typ2 (typ2 tyString tyVal) t0)
-         (typ2 tySubst (typ2 (typ2 tyString tyVal) t0))).
-      destruct (typ2_cast tySubst (typ2 (typ2 tyString tyVal) t0)).
-      unfold exprT_App.
-      simpl.
-      reflexivity.
-      unfold exprT_App. intros. simpl.
-      rewrite mkEmp_sound with (f := i).
-      setoid_rewrite mkEmp_sound.
-      eexists. split. erewrite mkEmp_sound.
-      erewrite mkEmp_sound.
-      Focus 3. eapply H3.
-      eexists. split.
-      eexists; split; [reflexivity|].
-      eexists.
-      split.
-      eapply mkEmp_sound; try eassumption.
-      rewrite mkEmp_sound.
-      Check mkEmp_sound.
-      eapply mkEmp_sound.
-      rewrite mkEmp_sound.
-      setoid_rewrite mkEmp_sound.
-      SearchAbout exprT_App.
-      unfold exprT_App. simpl.
-      eexists. split.
-      autorewrite with exprD_rw. simpl.
-      Print funcAs.
-      Print RType.
-      Print RSym.
-      Print funcAs.
-      unfold funcAs.
-      assert (typeof_sym (fEmp logic0) = Some logic0).  admit.
-      rewrite H4.
-      Print symD.
-      unfold symD. simpl.
-            Require Import Charge.Logics.BILogic.
-      SearchAbout typ2 typD.
-      Print Typ2_tyArr.
-      unfold exprT, OpenT. simpl.
-      rewrite (@typ2_cast typ RType_typ Fun Typ2_tyArr (typ2 tyString tyVal) t0).
-      unfold typ2. simpl. unfold exprT. simpl. unfold OpenT. simpl. unfold Ty
-      exists (fun _ _ => empSP).
-      
-      
-      try (solve [simpl; eexists; split; [eapply mkApplySubst_sound; eassumption|reflexivity]]).
-      Focus 2.
-      simpl; eexists; split; [|reflexivity].
-      Check @ilf_true_type_eq.
-      symmetry in Heqo0.
-      pose proof (ilf_true_type_eq (gs := gs) _ _ Heqo0 H3).
-      rewrite H4 in *; clear H4.
-      erewrite (mkTrue_sound (gs := gs)); [|eassumption|eassumption].
-      rewrite (ilf_funcAsOk _ Heqo0) in H3.
-      unfold funcAs in H3; simpl in H3. forward; inv_all; subst.
-      unfold Rcast, Relim, Rsym, eq_sym in H5. simpl in H5.
-      rewrite type_cast_refl in H4.
-      unfold Rrefl in H4; inv_all; subst.
-      inv_all; subst.
-      rewrite (of_funcAsOk _ Heqo) in H2.
-      pose proof (of_fApplySubstOk t0).
-      pose proof (OpenFunc_typeOk _ H4).
-      simpl in H5.
-      unfold funcAs in H2; simpl in H2.
-      rewrite type_cast_refl in H2.
-      inv_all; subst.
-      
-      (* Gregory: This should be true, but I don't quite know where to go from here. *)
-      
-      unfold exprT_App, fun3_wrap, fun2_wrap, fun1_wrap, fun1D, id, eq_rect_r, eq_rect. uip_all'.
-      
-      (* This gives me a bunch of equivalence proofs, and a lot of typing problems *)
-      
-      unfold Fun in *.
-      unfold exprT_App. simpl.
-      rewrite funcAs_Some with (pf := H5) in H2.
-      Check funcAs_Some.
-      Check OpenFunc_typeOk.
-      unfold funcAs in H2; simpl in H2; forward; inv_all; subst.
-      rewrite type_cast_refl in H2; inv_all; subst.
-      unfold Rcast, Rrefl in H4; simpl in H4; inv_all; subst.
-      unfold Rcast, Rrefl, Relim, Rsym, eq_sym, fun3_wrap, fun2_wrap, fun1_wrap, eq_rect, eq_rect_r, eq_rect, eq_sym, fun1D, eq_rect.
-      simpl.
-      unfold exprT_App, eq_sym.
-      forward.
-      simpl.
-      inv_all; subst.
-      clear H2 H4.
-      uip_all.
-      unfold Fun in e3.
-      subst.
-      uip_all.
-      unfold id.
-      generalize dependent (typD (typ2 tyString tyVal)).
-      destruct e1.
-      uip_all'.
-      destruct stSubst.
-      destruct ( typ2_cast (typ2 tyString tyVal) t0).
-      forward.
-      SearchAbout typ2_cast.
-      unfold typ2_cast in H2.
-      rewrite type_cast_refl in H2.
-      inversion H2; subst. f_equal.
-      unfold exprT_App, fun3_wrap, eq_sym. simpl.
-      apply functional_extensionality. intros.
-      apply functional_extensionality. intros.
-      Check of_funcAsOk.
-      rewrite mkTrue_sound.
-      assert (exprD' tus tvs
-      try (solve [simpl; eexists; split; [apply mkApplySubst_sound | reflexivity]; assumption]).
-    simpl.
-    assumption.
-    assumption.
-    + simpl. eexists; split; [|reflexivity].
-      apply mkApplySubst_sound; assumption.
-    + simpl; eexists; split; [|reflexivity].
-      apply mkApplySubst_sound; assumption.
-    + 
-      autorewrite with exprD_rw in H3; simpl in H3; forward; inv_all; subst.
-      unfold Rty in r. subst.
-      unfold mkApplySubst. simpl.
-      autorewrite with exprD_rw; simpl; forward; inv_all; subst.
-      autorewrite with exprD_rw; simpl; forward; inv_all; subst.
-      pose (nth_error_get_hlist_nth_Some _ H3).
-      destruct e as [? ?].
-      rewrite x.
-      autorewrite with exprD_rw; simpl; forward; inv_all; subst.
-      rewrite type_cast_refl.
-      unfold Rcast_val, Rrefl, Rcast, Relim, Rsym, eq_sym; simpl.
-      assert (open_funcS (fApplySubst t0) = Some (of_apply_subst t0)) by admit.
-      assert (typeof_sym (of_apply_subst t0) = Some (typ2 (typ2 (typ2 tyString tyVal) t0)
-                   (typ2 tySubst (typ2 (typ2 tyString tyVal) t0)))) by admit.
-      pose proof (funcAsOk _ H3); rewrite H7.
-      pose proof (funcAs_Some _ H6).
-      rewrite H8. simpl.
-      f_equal. f_equal. f_equal.
-      Require Import FunctionalExtensionality.
-      apply functional_extensionality. intros.
-      apply functional_extensionality. intros.
-      clear -H6.
-      revert H6.
-      generalize (symD (of_apply_subst t0)).
-      intros.
-      admit.
-      apply _.
-    + eexists; split; [|reflexivity].
-      
-      simpl.
-      Check symD.
-      Print typD.
-      Print RType.
-      Check exprT_App.
-      Print exprT.
- 
-Check @exprT_App.
-
-    generalize dependent (
-       (typ2 (typ2 (typ2 tyString tyVal) t)
-          (typ2 tySubst (typ2 (typ2 tyString tyVal) t)))).
-    generalize dependent (typD t0).
-    destruct z.
-    generalize dependent (typeof_sym (of_apply_subst t)).
-    rewrite H2.
-    destruct H2.
-    f_e
-    rewrite H.
-      progress autorewrite with exprD_rw; simpl; forward; inv_all; subst.
-      autorewrite with exprD_rw; simpl; forward; inv_all; subst.
-      
-      pose (nth_error_get_hlist_nth_Some _ H3).
-      destruct e as [? ?].
-      rewrite x.
-      autorewrite with exprD_rw; simpl; forward; inv_all; subst.
-      rewrite type_cast_refl.
-      unfold Rcast_val, Rrefl, Rcast, Relim, Rsym, eq_sym; simpl.
-      assert (open_funcS (fApplySubst t0) = Some (of_apply_subst t0)) by admit.
-      assert (typeof_sym (of_apply_subst t0) = Some (typ2 (typ2 (typ2 tyString tyVal) t0)
-                   (typ2 tySubst (typ2 (typ2 tyString tyVal) t0)))) by admit.
-      pose proof (funcAsOk _ H3); rewrite H7.
-      pose proof (funcAs_Some _ H6).
-      rewrite H8. simpl.
-      f_equal. f_equal. f_equal.
-      Require Import FunctionalExtensionality.
-      apply functional_extensionality. intros.
-      apply functional_extensionality. intros.
-      clear -H6.
-      revert H6.
-      generalize (symD (of_apply_subst t0)).
-      intros.
-      admit.
-      apply _.    
-      generalize  (typ2 (typ2 (typ2 tyString tyVal) t0)
-            (typ2 tySubst (typ2 (typ2 tyString tyVal) t0))).
-      generalize dependent (Some (typ2 (typ2 (typ2 tyString tyVal) t0)
-          (typ2 tySubst (typ2 (typ2 tyString tyVal) t0)))); intros; subst; reflexivity.
-      generalize (symD (of_apply_subst t0)).
-      intros. 
-      generalize dependent H6.
-      generalize dependent (Some (typ2 (typ2 (typ2 tyString tyVal) t0)
-          (typ2 tySubst (typ2 (typ2 tyString tyVal) t0)))); intros; subst; reflexivity.
-      generalize dependent H6.
-      uip_all.
-      subst.
-      destruct H6.
-      generalize dependent H6. uip_all'.
-      assert (symD (fApplySubst t0) = symD (of_apply_subst t0)).
-      assert (typo
-        Print symAs_Some.
-      
-      pose proof (funcAsOk _ H3). rewrite H6.
-      SearchAbout exprD' symD.
-      SearchAbout symD.
-
-      
-      Check symD.
-      SearchAbout funcAs symD.
-      Check funcAs.
-      
-      Print exprT_App.
-      assert (funcAs (fApplySubst t0)
-        (typ2 (typ2 (typ2 tyString tyVal) t0)
-           (typ2 tySubst (typ2 (typ2 tyString tyVal) t0))) = symD (of_apply_subst t0)).
-      destruct o.
-      admit.
-      unfold funcAs in Heqo0.
-      simpl in Heqo0.
-      admit.
-      assert False.
-      rewrite H3 in Heqo0.
-      forward.
-      rewrite H3.
-      rewrite type_cast_refl.
-      assert (open_funcS (fApplySubst t0) = Some (of_apply_subst t0)).
-      admit.
-      pose (funcAsOk _ H3). 
-      Check typeof_funcAs.
-      
-      rewrite e; clear e.
-      pose proof (OpenFunc_typeOk _ H3).
-      simpl.
-      unfold fApplySubst. simpl.
-      unfold funcAs.
-      simpl.
-      Transparent symD.
-      simpl.
-      SearchAbout nth_error nth_error_get_hlist_nth.
-      unfold nth_error.
-      progress autorewrite with exprD_rw; simpl; forward; inv_all; subst.
-      simpl in H3.
-    Check expr_strong_ind.
-    Check (fun (_ : HList.hlist typD tus) (_ : HList.hlist typD tvs) =>
-         symD (of_apply_subst t0)).
-    Check (fun (_ : HList.hlist typD tus) (_ : HList.hlist typD tvs) =>
-         @apply_subst).
-    Transparent symD.
-    simpl.
-    unfold fun3_wrap, fun2_wrap, eq_rect_r, eq_rect, eq_sym. simpl.
-    rewrite (@typ2_cast typ _ Fun _).
-    rewrite typ2_cast.
-    SearchAbout exprT_App.
-    unfold eq_rect_r, eq_rect, eq_sym.
-    SearchAbout typ2_cast.
-    Check @typ2_cast.
-    remember (typ2_cast (typ2 (typ2 tyString tyVal) t0)
-               (typ2 tySubst (typ2 (typ2 tyString tyVal) t0))).
-    destruct e1.
-    unfold typ2_cast.
-    Transparent symD. 
-    simpl.
-    refine (exists val' : exprT tus tvs (typD (typ2 (typ2 tyString tyVal) t0)),
-  ExprDsimul.ExprDenote.exprD' tus tvs (typ2 (typ2 tyString tyVal) t0)
-    (pushSubst Typ2_tyArr e0 e t0) = Some val' /\
-  (forall (us : HList.hlist typD tus) (vs : HList.hlist typD tvs),
-   P us vs ->
-   exprT_App
-     (exprT_App
-        _ e4) e2 us vs = val' us vs)).
-    simpl.
-    erewrite typ2_cast.
-    generalize dependent t3.
-    Transparent symD.
-    rewrite typ2_cast.
-    Print symD.
-    simpl in H2.
-    Example test t0 : exists x, x = typD (typ2 (typ2 (typ2 tyString tyVal) t0)
-          (typ2 tySubst (typ2 (typ2 tyString tyVal) t0))).
-    Proof.
-      repeat rewrite typ2_cast.
-      unfold Fun.
-      repeat rewrite btString.
-      rewrite stVal.
-      vm_compute.
-      destruct RType_typ. simpl.
-      destruct Typ2_tyArr.
-      simpl.
-      destruct BT. simpl. destruct ST. simpl.
-      SearchAbout typ2.
-      repeat rewrite typ2_cast.
-      unfold Fun. simpl.
-      destruct BT.
-      rewrite btString.
-    unfold funcAs in H2; simpl in H2.
-    rewrite type_cast_refl in H2.
-    unfold Rcast, Relim, Rrefl in H2. simpl in H2.
-    unfold eq_rect_r, eq_rect, Fun, eq_sym, eq_rect_r, typ2_cast in H2; simpl in H2.
-    destruct Typ2_tyArr; simpl in H2.
-    SearchAbout typ2_cast.
-    Print Typ2Ok.
-    Print typ2_match.
-    rewrite typ2_match_Proper in H2.
-    progress unfold typ2_cast in H2.
-    Print Rcast.
-    inv_all; subst.
-    unfold exprT_App, eq_sym, typ2_cast, exprT, OpenT, typ2_cast; simpl.
-    
-    rewrite type_cast_refl in H2.
-    SearchAbout Typ2.
-    unfold Rcast, Rrefl, eq_rect_r, eq_sym, eq_rect, typ2_cast in H2; simpl in H2.
-    
-    unfold Rcast, Rrefl, eq_rect_r, eq_sym, typ2_cast, Fun, eq_rect in H2; simpl in H2.
-    destruct Typ2_tyArr. simpl in H2.
-    unfold typD in H2. simpl in H2.
-    destruct RType_typ; simpl in *.
-    forward.
-    inv_all; subst.
-    unfold exprT_App, eq_sym. simpl.
-    uip_all'.
-    uip_all'.
-    destruct e3.
-    uip_all'.
-    revert H2. uip_all.
-    unfold eq_rect in H2.
-    inv_all; subst.
-    vm_compute in H2.
-    subst.
-    rewrite H8 in *.
-    inversion H7.
-    rewrite H7 in H2.
-    simpl in H4.
-    unfold typ2 in H2. simpl in H2.
-    destruct Typ2_tyArr.
-    simpl.
-    unfold typ2 in H2.
-    unfold funcAs in H2. simpl in H2.
-    forward.
-    generalize dependent t3.
-    subst.
-    unfold Rty in r.
-    rewrite <- r.
-    unfold Rcast, Relim, Rsym, eq_sym, eq_rect_r, eq_rect, eq_sym, typ2_cast, Fun, typD in H2; simpl in H2.
-    destruct RType_typ; simpl in *.
-    
-     destruct r.
-    simpl in H4.
-    unfold type_cast in H2. simpl in H2.
-    destruct RType_typ.
-    destruct r.
-    rewrite OpenFunc_typeOk in .
-    pose proof (
-       
-    assert (typeof_sym f = typeof_open_func _ (of_apply_subst t0)) by admit.
-    Check symD.
-    Check exprD.
-    Print RSymOk.
-    Print exprD'.
-    Print Expr.
-    Print exprT.
-    Print OpenT.
-    assert (funcAs f (typeof_open_func _ (of_apply_subst t0)) = 
-       Some (fun _ _ => @apply_subst (typD tyString) (typD tyVal) (typD t0))).
-    assert (funcAs ).
-    simpl in H4.
-    pose proof (typeof_funcAs H2) as H5.
-    rewrite H5 in H4; clear H5; inv_all; subst.
-
-
-    eexists; split; [|intros; reflexivity].
-
-    induction e using expr_strong_ind.
-    + simpl.
-    SearchAbout exprT_App.
-    
-    unfold exprT_App. simpl.
-    unfold exprT, OpenT. simpl.
-    split.
-    Focus 2.
-    intros. reflexivity.
-    exists e2.
-    + simpl in H0.
-      unfold exprT_App. simpl.
-      unfold exprT. simpl. unfold OpenT. simpl.
-      SearchAbout typ2_cast.
-    generalize dependent t3.
-    generalize dependent t2.
-    generalize dependent t1.
-    generalize dependent t.
-    generalize dependent tus.
-    generalize dependent tvs.
-    generalize dependent e.
-    generalize dependent e0.
-    subst.
-    rewrite H4.
-    remember (typeof_sym f).
-    rewrite H4 in H2.
-    simpl in H4. 
-    Check @UIP_refl.
-    revert H2 Heqo.
-    uip_all.
-    generalize dependent t3.
-    generalize dependent t2. generalize dependent t1. generalize dependent t.
-    generalize dependent tus. generalize dependent tvs. generalize dependent e.
-    generalize dependent e0.
-    symmetry in H4. setoid_rewrite <- H4.
-     generalize dependent func.
-    setoid_rewrite H4.
-     rewrite H4.
-    red in H4.
-    rewrite (@UIP_refl (option typ) _ _ H4) in H2.
-    U
-    Check UIP_rewrite.
-    UIP_rewrite
-    rewrite H4 in H2.
-    simpl. unfold typ2. simpl. unfold typ2. simpl.
-    destruct f. simpl in Heqo.
-    unfold funcAs in H2. simpl in H2.
-    unfold exprT_App, OpenT; simpl. uip_all.
-    rewrite (UIP_refl e1).
-	simpl in H. red_exprD.
-	Locate idred.
-Check idred.
-*)
-Print full_reducer.
+		  unfold applySubstD, wandD, fun_to_typ2, fun_to_typ3; repeat rewrite exprT_App_wrap. 
+	      rewrite <- H12, <- H14.
+		  unfold applySubstD, fun_to_typ3; repeat rewrite exprT_App_wrap.
+		  admit.
+		}
+      }
+    }
+  }
+}
+Time Qed.
+	      
+	    
   Definition SUBST := SIMPLIFY (typ := typ) (fun _ _ _ _ => beta_all substTac).
-(*
-  Lemma substTac_ok : full_reducer_ok substTac.
-  Proof.
-    unfold full_reducer_ok; intros.
-    SearchAbout exprT.
-    Print OpenT.
-    unfold exprT, OpenT in *.
-Check hlist_build.
-SearchAbout apps.
-Print apps_sem'.
-Print apply_sem'.
-Check apps_sound.
-    Print var_termsP.
-    unfold applys. simpl.
-  Lemma substTac_sound   
-    (He : exprD' tus tvs (fold_right (typ2 (F := Fun)) t targs) e = Some de) :
-    exists de', exprD' tus' tvs' t (substTac var_terms e es) = Some de'
-    SearchAbout 
-    unfold OpenT.
-  Qed.
-Check @SIMPLIFY_sound.
-  Lemma SUBST_sound : @rtac_sound typ (expr typ func) RType_typ _ Expr_expr _ SUBST.
-  Proof.
-    unfold SUBST.
-    apply SIMPLIFY_sound.
-    intros; simpl; forward.
-    unfold propD, exprD'_typ0 in H3. forward; inv_all; subst.
-    destruct (beta_all_sound substTac_ok _ _ e1 H3) as [v [H4 H5]].
-    unfold propD, exprD'_typ0; simpl.
-    forward; inv_all; subst.
-    SearchAbout typ0_cast.
-    uip_all.
-    Check Pure_pctxD.
-    eapply Pure_pctxD; eauto.
-    intros us0 vs0; autorewrite with eq_rw. intro; rewrite H5. tauto.
-    assumption.
-  Qed.
-*)
+
   
 End SubstTac.
 Print SUBST.
